Update pure_anfTheory to work with cexp, first draft for the A-normalization algorithm

compiler/backend/pure_anfScript.sml
@@ -4,56 +4,304 @@
 open HolKernel Parse boolLib bossLib term_tactic;
 open fixedPointTheory arithmeticTheory listTheory stringTheory alistTheory
      optionTheory pairTheory ltreeTheory llistTheory bagTheory dep_rewrite
-     BasicProvers pred_setTheory relationTheory rich_listTheory finite_mapTheory;
+     BasicProvers pred_setTheory relationTheory rich_listTheory finite_mapTheory
+     state_transformerTheory ASCIInumbersTheory;
+
+
 open pure_expTheory pure_exp_lemmasTheory mlmapTheory mlstringTheory
-     pure_varsTheory;
+     pure_cexpTheory pure_varsTheory pure_beta_equivTheory;
 
 val _ = new_theory "pure_anf";
 
-
 (* definition of ANF syntax *)
 
-Datatype:
-  anf = Var vname                            (* var *)
-      | If vname anf anf                     (* if *)
-      | Seq (*intentional:*)exp anf          (* exp strict in rest *)
-      | Let vname op (vname list) anf        (* let v = op vars in rest *)
-      | LetApp vname vname (vname list) anf  (* let v = f vars in rest *)
-      | LetLam vname (vname list) anf anf    (* non-recursive function *)
-      | Letrec ((vname # anf) list) anf      (* recursive bindings *)
-End  (* above, note that, in the Let case, op should not be If or Seq *)
+(*What it should be:
+  value  = Var vname
+         | Lam (vname list) anf;
 
-Triviality anf_size_lemma:
-  ∀xs n x. MEM (n,x) xs ⇒ anf_size x ≤ anf1_size xs
+  canf   = App value (value list)
+         | Prim op (value list)
+         | Case vname ((string # vname list # anf) list);
+
+  anf    = Let vname canf anf
+         | Letrec ((vname # canf) list) anf
+         | canf
+         | value;
+
+  this shape reflect the intrinsic property of A-normal form expressions:
+  anf expressions are either:
+   - values
+   - Lambdas/primitives applied to values (App/Prim/Case (If primitive))
+   - let binds (Let/Letrec)
+*)
+
+(*
+  What actually is to avoid mutual recursion:
+*)
+
+Datatype:
+  anf    = Var 'a vname
+         | Lam 'a (vname list) anf
+         | App 'a anf (anf list)
+         | Prim 'a cop (anf list)
+         | Case 'a vname ((string # vname list # anf) list)
+         | Let 'a vname anf anf
+         | Letrec 'a ((vname # anf) list) anf
+End
+
+(*avoiding mutual recursion is a bad idea. The proper datatype
+  definition forces the anf expressions to comply with the A-normal
+  form intrinsic property (above).
+  This relieves us from proving ‘anf_of’ actually produces
+  A-normal form expressions (I think).
+*)
+
+Definition is_value_def:
+    (is_anf_value (Var _ _) = T)
+  ∧ (is_anf_value (Lam _ _ _) = T)
+  ∧ (is_anf_value _ = F)
+End
+
+Definition get_anf_annotation_def:
+    get_anf_annotation (Var a _)      = a
+  ∧ get_anf_annotation (Lam a _ _)    = a
+  ∧ get_anf_annotation (App a _ _)    = a
+  ∧ get_anf_annotation (Prim a _ _)   = a
+  ∧ get_anf_annotation (Case a _ _)   = a
+  ∧ get_anf_annotation (Let a _ _ _)  = a
+  ∧ get_anf_annotation (Letrec a _ _) = a
+End
+
+Theorem anf_size_lemma:
+  (∀ xs n x. MEM (n,x) xs ⇒ anf_size (K 0) x ≤ anf4_size (K 0) xs) ∧
+  (∀cases as b. MEM (c,as,b) cases ⇒ anf_size (K 0) b ≤ anf1_size (K 0) cases) ∧
+  (∀ xs n x. MEM x xs ⇒ anf_size (K 0) x ≤ anf6_size (K 0) xs)
 Proof
-  Induct \\ ntac 2 (rw [fetch "-" "anf_size_def"]) \\ res_tac \\ fs []
+  rpt CONJ_TAC
+  \\ Induct \\ ntac 2 (rw [fetch "-" "anf_size_def"]) \\ res_tac \\ fs []
 QED
 
+(* we use ANF as rigid way of writing normal pure_lang cexp expressions *)
 
-(* we use ANF as rigid way of writing normal pure_lang expressions exp *)
-
-Definition Apps_def:
-  Apps f [] = f ∧
-  Apps f (x::xs) = Apps (App f x) xs
-End
-
-Definition Lams_def:
-  Lams [] b = b ∧
-  Lams (x::xs) b = Lam x (Lams xs b)
-End
-
-Definition exp_of_def:
-  exp_of ((Var v) : anf)   = ((Var v):exp) ∧
-  exp_of (If v x y)        = If (Var v) (exp_of x) (exp_of y) ∧
-  exp_of (Seq e x)         = Seq e (exp_of x) ∧
-  exp_of (Let v p vs x)    = Let v (Prim p (MAP Var vs)) (exp_of x) ∧
-  exp_of (LetApp v f vs x) = Let v (Apps (Var f) (MAP Var vs)) (exp_of x) ∧
-  exp_of (LetLam v vs b x) = Let v (Lams vs (exp_of b)) (exp_of x) ∧
-  exp_of (Letrec xs y)     = Letrec (MAP (λ(n,x). (n, exp_of x)) xs) (exp_of y)
+Definition cexp_of_def:
+  cexp_of (Var d x) = (Var d x) ∧
+  cexp_of (Lam d args b) = Lam d args (cexp_of b) ∧
+  cexp_of (App d f args) = App d (cexp_of f) (MAP cexp_of args) ∧
+  cexp_of (Prim d cop args) = Prim d cop (MAP cexp_of args) ∧
+  cexp_of (Case d v cases) =
+       Case d v (MAP (λ(n,as,b).(n,as,cexp_of b)) cases)  ∧
+  cexp_of (Let d v a b) = Let d v (cexp_of a) (cexp_of b) ∧
+  cexp_of (Letrec d binds body) =
+       Letrec d (MAP (λ(v,e).(v,cexp_of e)) binds) (cexp_of body)
 Termination
-  WF_REL_TAC ‘measure anf_size’ \\ rw []
+  WF_REL_TAC ‘measure (anf_size (K 0))’ \\ rw []
   \\ imp_res_tac anf_size_lemma \\ fs []
 End
+
+val _ = monadsyntax.enable_monadsyntax () ;
+monadsyntax.enable_monad "state";
+
+
+(*state for the normalization algorithm.
+  Keeps track of an index used to generate new fresh variables.
+*)
+Datatype:
+  anf_state = <| base        : vname
+               ; vname_index : int    |>
+End
+
+(*State monad (with state fixed: ‘anf_state’)*)
+Type S[local] = “:anf_state -> ('a # anf_state)”;
+
+(*Continuation function type (not a monad)*)
+Type CONT[local] = “:('a anf -> ('a anf) S)”;
+
+Definition new_vname_def:
+  new_vname : (vname) S = do
+          i <- READ (anf_state_vname_index);
+          base <- READ (anf_state_base);
+          WRITE (λ s. s with vname_index updated_by ($+ 1));
+          return (base++toString i);
+       od
+End
+
+(*takes a continuation k, returns a continuation that
+  grabs the returning value (anf_e):
+    if is a value (Val or Lam)
+      then passes it to k
+      else binds it to a fresh variable (t)
+           and passes (Var t) to k
+*)
+Definition let_bind_def:
+   let_bind : 'a CONT -> 'a CONT
+              k = (λ anf_e.
+                     if (is_anf_value anf_e)
+                       then k anf_e
+                       else (let an_e = get_anf_annotation anf_e in
+                               do t <- new_vname ;
+                                  anf_res <- k (Var an_e t) ;
+                                  return $ Let an_e t anf_e anf_res
+                               od))
+End
+
+(*A-normalization algorithm for cexp expressions.
+  Originally from https://dl.acm.org/doi/10.1145/173262.155113*)
+Definition normalize_def:
+  (* normalize : 'a cexp -> ('a CONT) -> ('a anf) S *)
+  (*values, call k on them*)
+    (normalize (Var d x : 'a cexp) (k: 'a CONT) =
+         k ((Var d x) : 'a anf))
+  ∧ (normalize (Lam d args body)   (k: 'a CONT) = do
+         anf_b <- (normalize body (return)) ;
+         k $ Lam d args anf_b
+      od)
+  (*exprs*)
+  ∧ (normalize (Let d v a b) (k: 'a CONT) =
+         normalize a (λ anf_a.
+             do anf_b <- (normalize b k) ;
+                return $ Let d v anf_a anf_b
+             od ))
+  ∧ (normalize ((Case d e v cases):'a cexp) (k: 'a CONT) =
+         normalize e $ let_bind (λ anf_e.
+            do anf_cases <- mapM (λ(n,args,body). do
+                                    anf_b <- normalize body (return) ;
+                                    return $ (n,args,anf_b) ;
+                                  od) cases;
+               return $ Let d v anf_e (Case d v anf_cases)
+             od ))
+  ∧ (normalize (App  d f  es) (k : 'a CONT) =
+         normalize f $ let_bind (λ anf_f.
+            normalize_names es (λ anf_es.
+                      k (App d anf_f anf_es))))
+  ∧ (normalize (Prim d op es) (k : 'a CONT) =
+         normalize_names es (λ anf_es.
+             k (Prim d op anf_es)))
+  ∧ (normalize (pure_cexp$Letrec d binds body) (k : 'a CONT) =
+         normalize body (λ anf_body.
+            do anf_binds <- mapM (λ(n,f). do
+                                   anf_f <- normalize f (return) ;
+                                   return $ (n,anf_f) ;
+                                od) binds;
+               return (Letrec d anf_binds anf_body)
+            od ))
+    (* normalize_name e k = normalize e (let_bind k) *)
+  ∧ (normalize_names [] k = k [])
+  ∧ (normalize_names (e::es) k = normalize e $ let_bind (λ anf_e.
+                               normalize_names es (λ anf_es.
+                                 k (anf_e::anf_es))))
+Termination
+  cheat
+End
+
+(*
+    (* TODO: removing mutual recursion from normalize_def*)
+
+    (* normalize_names [] k = k [] *)
+    (* normalize_names (e::es) k = normalize e $ let_bind (λ anf_e.
+                               normalize_names es (λ anf_es.
+                                 k (anf_e::anf_es))) *)
+    (*move k to rhs*)
+
+    normalize_names [] k = k []
+    normalize_names (e::es) k = normalize e $ let_bind (λ anf_e.
+                               normalize_names es (λ anf_es.
+                                 k (anf_e::anf_es)))
+
+    (* (λ anf_es. k (anf_e::anf_es)) ≡ (k o (CONS anf_e)) *)
+
+    normalize_names [] = (λ k. k []) (*base case*)
+    normalize_names (e::es) = (*fold step*)
+        (λ k. normalize e $
+               let_bind (λ x. normalize_names es (k o (CONS x))))
+
+    (* ??? *)
+
+    normalize_names es =
+        FOLDR (λ e r. (λ k. normalize e $
+                             let_bind (λ x. r (k o (CONS x)))))
+              (λ k. k []) es
+
+    (*eta-contraction*)
+
+    normalize_names =
+       FOLDR (λ e r. (λ k. normalize e $
+                             let_bind (λ x. r (k o (CONS x)))))
+             (λ k. k [])
+*)
+
+
+
+Definition fresh_state_def:
+  fresh_state s avoid
+    ⇔ s.base ∉ avoid ∧ (∀ ss. (STRCAT s.base ss) ∉ avoid)
+End
+
+(*given a fresh starting state, new_vname produces a fresh vname*)
+Theorem new_vname_freshness:
+  ∀ s avoid. fresh_state s avoid
+         ⇒ FST (new_vname s) ∉ avoid
+Proof
+  rw[] \\ fs[fresh_state_def,new_vname_def]
+  \\ EVAL_TAC \\ rw[] \\ fs[]
+QED
+
+(*new_vname does not alter the freshness of the state*)
+Theorem new_vname_fresh_state_mono:
+  ∀ s avoid. fresh_state s avoid
+           ⇒ fresh_state (SND (new_vname s)) avoid
+Proof
+  rw[] \\ fs[fresh_state_def,new_vname_def]
+  \\ EVAL_TAC \\ fs[]
+QED
+
+Definition fresh_var_substr_def:
+   fresh_var_substr v avoid =
+       if(¬MEM v avoid ∧ FOLDR MAX 0 (MAP LENGTH avoid) < LENGTH v)
+           then v
+           else (fresh_var_substr (v ++ "'") avoid)
+Termination
+  WF_REL_TAC ‘measure (λ(v,xs). (LENGTH (FLAT xs) + 1) - LENGTH v)’
+  \\ Induct \\ fs[] \\ rw[] \\ fs[] \\ res_tac \\ fs[]
+End
+
+Theorem fresh_var_substr_correctness:
+   ∀ v l. let x = fresh_var_substr v l
+          in ¬MEM x l ∧ (∀ ss. ¬MEM (STRCAT x ss) l)
+Proof
+  recInduct fresh_var_substr_ind \\ rw[] \\ fs[]
+  \\ once_rewrite_tac [fresh_var_substr_def]
+  \\ IF_CASES_TAC \\ fs[]
+  \\ CCONTR_TAC \\ fs[]
+  \\ Induct_on ‘avoid’ \\ fs[]
+QED
+
+Definition start_state_def:
+  start_state e =
+      <| base  :=
+         fresh_var_substr ".res_" (  freevars_l  (exp_of e)
+                                  ++ boundvars_l (exp_of e))
+       ; vname_index := 0
+       |>
+End
+
+Triviality start_state_fresh_state:
+  ∀ e. fresh_state
+           (start_state e)
+           (freevars (exp_of e) ∪ boundvars (exp_of e))
+Proof
+  rw[]
+  \\ fs[fresh_state_def,start_state_def]
+  \\ qspecl_then [‘".res_"’
+                 ,‘freevars_l (exp_of e) ++ boundvars_l (exp_of e)’]
+                 mp_tac fresh_var_substr_correctness
+  \\ fs[freevars_equiv,boundvars_equiv]
+QED
+
+Definition anf_of_def:
+  anf_of e = normalize e (return) (start_state e)
+End
+
+
 
 (*
 
@@ -68,17 +316,6 @@ implementation of the compiler.
 Every Let in the generated anf ought to bind a unqiue name. Ideally,
 all new names should have a recognisable prefix like "." so that we
 can easily see which names are generated.
-
-Note that LetApp and LetLam should try to maximize the number of
-arguments, e.g.
-
-  LetApp v f [x; y; z] rest
-
-instead of:
-
-  LetApp v f [x] (LetApp v' v [y] (LetApp v'' v' [z] rest))
-
-Similarly LetLam should bind as many variables as possible in the Lam.
 
 The following should also hold:
 
